theories/Core/Soundness/ContextCases.v
@@ -3,7 +3,7 @@ From Coq Require Import Morphisms Morphisms_Prop Morphisms_Relations Relation_De
 From Mcltt Require Import Base LibTactics.
 From Mcltt.Core.Completeness Require Import FundamentalTheorem.
 From Mcltt.Core.Semantic Require Import Realizability.
-From Mcltt.Core.Soundness Require Import LogicalRelation Realizability.
+From Mcltt.Core.Soundness Require Import LogicalRelation.
 From Mcltt.Core.Syntactic Require Import Corollaries.
 Import Domain_Notations.
 
@@ -18,27 +18,13 @@ Hint Resolve glu_rel_ctx_empty : mcltt.
 Lemma glu_rel_ctx_extend : forall {Γ A i},
     {{ ⊩ Γ }} ->
     {{ Γ ⊩ A : Type@i }} ->
-    {{ ⊩ Γ , A }}.
+    {{ ⊩ Γ, A }}.
 Proof.
   intros * [Sb] HA.
-  destruct (invert_glu_rel_exp ltac:(eassumption) HA) as [].
+  assert {{ Γ ⊢ A : Type@i }} by mauto.
+  invert_glu_rel_exp HA.
   eexists.
   econstructor; mauto; try reflexivity.
-  intros.
-  (* TODO: extract this as a tactic *)
-  repeat match goal with
-         | H: context[glu_rel_exp_sub _ _ _ _ _ _] |- _ =>
-             match type of H with
-             | __mark__ _ _ => fail 1
-             | _ => edestruct H; try eassumption; mark H
-             end
-         end; unmark_all.
-  simplify_evals.
-  match_by_head glu_univ_elem ltac:(fun H => directed invert_glu_univ_elem H).
-  handle_functional_glu_ctx_env.
-  unfold univ_glu_exp_pred' in *.
-  destruct_conjs.
-  econstructor; mauto.
 Qed.
 
 #[export]
