theories/Core/Soundness/SubstitutionCases.v
@@ -43,22 +43,17 @@ Lemma glu_rel_sub_compose : forall {Γ1 σ2 Γ2 σ1 Γ3},
     {{ Γ1 ⊩s σ1 ∘ σ2 : Γ3 }}.
 Proof.
   intros * Hσ2 Hσ1.
-  pose proof Hσ2 as [SbΓ1 [SbΓ2]].
-  destruct_conjs.
-  destruct (invert_glu_rel_sub1 ltac:(eassumption) Hσ1) as [SbΓ3].
-  destruct_conjs.
-  do 2 eexists; repeat split; mauto.
-  intros.
-  repeat match reverse goal with
-         | H: context[glu_rel_sub_sub _ _ _ _ _] |- _ =>
-             match type of H with
-             | __mark__ _ _ => fail 1
-             | _ => edestruct H; try eassumption; mark H
-             end
-         end; unmark_all.
-  econstructor; mauto.
   assert {{ Γ2 ⊢s σ1 : Γ3 }} by mauto.
   assert {{ Γ1 ⊢s σ2 : Γ2 }} by mauto.
+  destruct Hσ2 as [SbΓ1 [SbΓ2]].
+  destruct_conjs.
+  invert_glu_rel_sub Hσ1.
+  do 2 eexists; repeat split; mauto.
+  intros.
+  destruct_glu_rel_sub_sub.
+  destruct_glu_rel_sub_sub.
+  handle_functional_glu_ctx_env.
+  econstructor; mauto.
   enough {{ Δ ⊢s (σ1 ∘ σ2) ∘ σ ≈ σ1 ∘ (σ2 ∘ σ) : Γ3 }} as -> by eassumption.
   mauto 3.
 Qed.
@@ -73,43 +68,33 @@ Lemma glu_rel_sub_extend : forall {Γ σ Δ M A i},
     {{ Γ ⊩s (σ ,, M) : Δ , A }}.
 Proof.
   intros * Hσ HA HM.
-  pose proof Hσ as [SbΓ [SbΔ]].
+  assert {{ Γ ⊢s σ : Δ }} by mauto 3.
+  assert {{ Δ ⊢ A : Type@i }} by mauto 3.
+  assert {{ Γ ⊢ M : A[σ] }} by mauto 3.
+  destruct Hσ as [SbΓ [SbΔ]].
   destruct_conjs.
-  unshelve epose proof (invert_glu_rel_exp _ HA) as [j]; shelve_unifiable; [eassumption |].
-  unshelve epose proof (invert_glu_rel_exp _ HM) as [k]; shelve_unifiable; [eassumption |].
+  invert_glu_rel_exp HA.
+  rename x into j.
+  invert_glu_rel_exp HM.
+  rename x into k.
   do 2 eexists; repeat split; mauto.
-  - assert {{ Δ ⊢ A : Type@(max i k) }} by mauto 4 using lift_exp_max_left.
+  - assert {{ Δ ⊢ A : Type@(max i k) }} by mauto 2 using lift_exp_max_left.
     econstructor; mauto 3; try reflexivity.
     intros.
-    repeat match reverse goal with
-           | H: context[glu_rel_exp_sub _ _ _ _ _ _] |- _ =>
-               match type of H with
-               | __mark__ _ _ => fail 1
-               | _ => edestruct H; [eassumption |]; mark H
-               end
-           end; unmark_all.
+    destruct_glu_rel_exp_sub.
     simplify_evals.
     match_by_head glu_univ_elem ltac:(fun H => directed invert_glu_univ_elem H).
     apply_predicate_equivalence.
     unfold univ_glu_exp_pred' in *.
     destruct_conjs.
     rename m into a.
-    assert (exists P El, {{ DG a ∈ glu_univ_elem (max i k) ↘ P ↘ El }}) as [? []] by mauto using glu_univ_elem_cumu_max_left.
-    econstructor; mauto.
+    assert {{ Dom a ≈ a ∈ per_univ i }} as [] by mauto.
+    eapply mk_glu_rel_typ_sub''; mauto using per_univ_elem_cumu_max_left.
+    intros.
     eapply glu_univ_elem_typ_cumu_max_left; revgoals; mautosolve.
   - intros.
-    repeat match reverse goal with
-           | H: context[glu_rel_exp_sub _ _ _ _ _ _] |- _ =>
-               match type of H with
-               | __mark__ _ _ => fail 1
-               | _ => edestruct H; [eassumption |]; mark H
-               end
-           | H: context[glu_rel_sub_sub _ _ _ _ _] |- _ =>
-               match type of H with
-               | __mark__ _ _ => fail 1
-               | _ => edestruct H; [eassumption |]; mark H
-               end
-           end; unmark_all.
+    destruct_glu_rel_sub_sub.
+    destruct_glu_rel_exp_sub.
     simplify_evals.
     match_by_head glu_univ_elem ltac:(fun H => directed invert_glu_univ_elem H).
     apply_predicate_equivalence.
@@ -120,7 +105,6 @@ Proof.
     assert {{ Δ ⊢ A : Type@i }} by mauto 3.
     assert {{ Γ ⊢s σ : Δ }} by mauto 3.
     assert {{ Δ0 ⊢s σ0 : Γ }} by mauto 4.
-    assert (exists P El, {{ DG a ∈ glu_univ_elem (max i k) ↘ P ↘ El }}) as [Pmax [Elmax]] by mauto 3 using glu_univ_elem_cumu_max_left.
     econstructor; mauto 3.
     assert {{ Δ0 ⊢s (σ,,M)∘σ0 : Δ, A }} by mauto 3.
     assert {{ Δ0 ⊢s (σ,,M)∘σ0 ≈ (σ∘σ0),,M[σ0] : Δ, A }} by mauto 3.
@@ -130,6 +114,7 @@ Proof.
     assert {{ Δ0 ⊢ M[σ0] : A[σ∘σ0] }} by mauto 3.
     assert {{ Δ0 ⊢s Wk∘((σ∘σ0),,M[σ0]) ≈ σ∘σ0 : Δ }} by mauto 3.
     assert {{ Δ0 ⊢s Wk∘((σ,,M)∘σ0) ≈ σ∘σ0 : Δ }} by mauto 3.
+    assert (exists P El, {{ DG a ∈ glu_univ_elem (max i k) ↘ P ↘ El }}) as [Pmax [Elmax]] by mauto 3 using glu_univ_elem_cumu_max_left.
     econstructor; mauto 4.
     + assert {{ Δ, A ⊢s Wk : Δ }} by mauto 4.
       assert {{ Δ0 ⊢ A[Wk][(σ,,M)∘σ0] ≈ A[Wk∘((σ,,M)∘σ0)] : Type@i }} by mauto 4.
