theories/LibTactics.v
@@ -88,7 +88,8 @@ Ltac find_dup_hyp tac non :=
   | [ H : ?X, H' : ?X |- _ ] =>
     not_let_bind H;
     not_let_bind H';
-    lazymatch type of X with
+    let T := type of X in
+    lazymatch eval cbv in T with
     | Prop => tac H H' X
     | _ => fail
     end
